case_study/RiscvPmp/BlockVer/PartialVerifier.v
@@ -686,7 +686,7 @@ Section AnnotatedBlockVerification.
     Import ProgramLogic.
     Import CHeapSpec.
 
-    Context {Σ} {GS : sailGS Σ}.
+    Context {Σ} {GS : sailGS Σ} {rG : trivGS Σ}.
 
     Definition extract_AST (i : AnnotInstr) : option AST :=
       match i with
